More progress on bytestring

verification/specs_general.v
@@ -16,6 +16,7 @@ From VeriFFI Require Export library.meta library.modelled.
 From VeriFFI Require Export verification.graph_add.
 (* From VeriFFI Require Export verification.example.glue. *)
 From VeriFFI Require Export verification.specs_library.
+Import spatial_gcgraph.
 
 (** ** 3. A General Specification *)
 
@@ -214,5 +215,417 @@ Ltac start_function' :=
   start_function2;
   start_function3.
 
+
+Lemma is_pointer_or_integer_rep_type_val:
+  forall {A} `{InG: InGraph A} g (n: A) p, 
+   is_in_graph g n p ->
+   graph_rep g |-- !! is_pointer_or_integer (rep_type_val g p).
+Proof.
+intros.
+destruct p; simpl; auto.
+destruct g0; simpl; auto.
+apply has_v in H.
+sep_apply (graph_rep_valid_int_or_ptr g v).
+entailer!!.
+hnf in H0|-*.
+destruct (vertex_address g v); auto.
+destruct Archi.ptr64; auto.
+Qed.
+
+Lemma before_gc_thread_info_rep_fold:
+  forall sh t_info (ti: val),
+  @data_at env_graph_gc.CompSpecs sh env_graph_gc.thread_info_type
+   (offset_val (WORD_SIZE * used_space (heap_head (ti_heap t_info))) (space_start (heap_head (ti_heap t_info))),
+    (offset_val (WORD_SIZE * total_space (heap_head (ti_heap t_info))) (space_start (heap_head (ti_heap t_info))),
+     (ti_heap_p t_info,
+      (ti_args t_info,
+        (spatial_gcgraph.ti_fp t_info, (Vptrofs (ti_nalloc t_info), nullval)))))) ti
+  * spatial_gcgraph.frames_rep sh (ti_frames t_info)
+  * spatial_gcgraph.heap_struct_rep sh
+      ((space_start (heap_head (ti_heap t_info)),
+       (Vundef,
+       (offset_val (WORD_SIZE * total_space (heap_head (ti_heap t_info))) (space_start (heap_head (ti_heap t_info))),
+         offset_val (WORD_SIZE * total_space (heap_head (ti_heap t_info))) (space_start (heap_head (ti_heap t_info))))))
+         :: map spatial_gcgraph.space_tri (tl (spaces (ti_heap t_info))))
+      (ti_heap_p t_info)
+  * spatial_gcgraph.heap_rest_rep (ti_heap t_info) 
+  |-- before_gc_thread_info_rep sh t_info ti.
+Proof.
+ intros.
+ unfold before_gc_thread_info_rep.
+ unfold spatial_gcgraph.before_gc_thread_info_rep.
+ cancel.
+Qed.
+
+
+Lemma frames_rep_cons:
+ forall sh vf vr vl frames
+  (SIZE: WORD_SIZE * Zlength vl <= Ptrofs.max_signed),
+ (frame_rep sh vf vr (spatial_gcgraph.frames_p frames) vl *
+  spatial_gcgraph.frames_rep sh frames)%logic
+ = spatial_gcgraph.frames_rep sh 
+     ({|fr_adr:=vf; fr_root:=vr; fr_roots := vl|}::frames).
+Proof.
+intros.
+unfold frame_rep.
+simpl.
+unfold tarray.
+unfold spatial_gcgraph.frames_rep.
+unfold frames2rootpairs.
+simpl map.
+change (concat (?A :: ?B)) with (A ++ concat B).
+fold (frames2rootpairs frames).
+unfold spatial_gcgraph.roots_rep.
+rewrite iter_sepcon.iter_sepcon_app_sepcon.
+unfold spatial_gcgraph.frames_shell_rep; fold (spatial_gcgraph.frames_shell_rep sh frames).
+unfold frame2rootpairs.
+simpl.
+match goal with |- ?A = ?B =>
+ transitivity (!! (@field_compatible0 env_graph_gc.CompSpecs (tarray int_or_ptr_type (@Zlength val vl)) [] vr) && A)%logic
+ end.
+   apply pred_ext; entailer!.
+ normalize.
+ apply andp_prop_ext. tauto.
+ intro.
+ rewrite spatial_gcgraph.iter_sepcon_frame2rootpairs' by auto.
+replace  (field_address0 (tarray int_or_ptr_type (Zlength vl)) (SUB Zlength vl) vr)
+with (offset_val (8 * Zlength vl) vr).
+2:{ unfold field_address0.
+  rewrite if_true. simpl. auto.
+   eapply field_compatible0_cons_Tarray; [ | apply H| ].
+   reflexivity. rep_lia.
+}
+apply pred_ext; cancel.
+Qed.
+
+Lemma frames_rep_push:
+ forall sh vf vr vl frames
+  (SIZE: WORD_SIZE * Zlength vl <= Ptrofs.max_signed),
+frame_rep sh vf vr (spatial_gcgraph.frames_p frames) vl *
+spatial_gcgraph.frames_rep sh frames
+|-- spatial_gcgraph.frames_rep sh 
+     ({|fr_adr:=vf; fr_root:=vr; fr_roots := vl|}::frames).
+Proof.
+intros.
+rewrite frames_rep_cons by auto. auto.
+Qed.
+
+
+Lemma frames_rep_pop:
+ forall sh vf vr vl frames
+  (SIZE: WORD_SIZE * Zlength vl <= Ptrofs.max_signed),
+ spatial_gcgraph.frames_rep sh 
+     ({|fr_adr:=vf; fr_root:=vr; fr_roots := vl|}::frames)
+|-- frame_rep sh vf vr (spatial_gcgraph.frames_p frames) vl *
+    spatial_gcgraph.frames_rep sh frames.
+Proof.
+intros.
+rewrite frames_rep_cons by auto. auto.
+Qed.
+
+
+Lemma headroom_check {cs: compspecs}: 
+ forall (n: Z) (hh: space) (startb: block) (starti: ptrofs),
+  Int.min_signed <= n <= Int.max_signed ->
+  typed_false tint
+       match
+         sem_unary_operation Onotbool tint
+           (force_val
+              (both_long
+                 (fun n1 n2 : int64 => Some (bool2val (negb (Int64.lt n2 n1))))
+                 (sem_cast_i2l Signed) sem_cast_pointer 
+                 (Vint (Int.repr n))
+                 (force_val
+                    (sem_sub_pp
+                       int_or_ptr_type
+                       (Vptr startb
+                          (Ptrofs.add starti
+                             (Ptrofs.repr
+                                (WORD_SIZE
+                                   * total_space hh))))
+                       (Vptr startb
+                          (Ptrofs.add starti
+                             (Ptrofs.repr
+                                (WORD_SIZE
+                                   * used_space hh))))))))
+       with
+       | Some v' => v'
+       | None => Vundef
+       end ->
+  total_space hh - used_space hh >= n.
+Proof.
+intros * H7 H8.
+    assert (ORDER := space_order hh).
+    assert (UB := space_upper_bound hh).
+    set (tot := total_space hh) in *. clearbody tot.
+    set (use := used_space hh) in *. clearbody use.
+    simpl in H8.
+    unfold sem_sub_pp in H8. simpl in *. rewrite if_true in H8 by auto. simpl in H8.
+     rewrite Int.signed_repr in H8 by auto.
+    destruct (Int64.lt _ _) eqn:?H in H8; try discriminate.
+    unfold Int64.lt in H.
+    if_tac in H; try discriminate. clear H H8.
+    rewrite !(Ptrofs.add_commut starti), Ptrofs.sub_shifted, ptrofs_sub_repr in H0.
+    unfold MAX_SPACE_SIZE in *. simpl in UB.
+    rewrite <- Z.mul_sub_distr_l in H0.
+    change WORD_SIZE with 8 in *.
+    rewrite ptrofs_divs_repr in H0 by rep_lia.
+    rewrite ptrofs_to_int64_repr in H0 by reflexivity.
+    rewrite Z.mul_comm, Z.quot_mul in H0 by lia.
+    rewrite !Int64.signed_repr in H0 by rep_lia. auto.
+Qed.
+
+
+
+Ltac sep_apply_compspecs cs H :=
+  generalize H; 
+  limited_change_compspecs cs; (* Bug?  If there's no compspecs at all in H or the goal,
+    then this fails, but perhaps in that case it should succeed. *)    
+  let Hx := fresh "Hx" in  intro Hx; sep_apply Hx; clear Hx.
+
+Lemma space_start_isptr':
+  forall [g tinfo roots outlier],
+  gc_condition_prop g tinfo roots outlier ->
+  isptr (space_start (heap_head (ti_heap tinfo))).
+Proof.
+ intros * GCP.
+    red in GCP; decompose [and] GCP.
+    destruct (heap_head_cons (ti_heap tinfo)) as [s [l [C1 C2]  ] ].
+    rewrite C2.
+    replace s with (Znth 0 (spaces (ti_heap tinfo))) by (rewrite C1; reflexivity).
+    apply space_start_isptr with g; auto; try apply H1.
+    rewrite C1; clear; list_solve.
+    apply graph_has_gen_O.
+Qed.
+
+Local Open Scope logic.
+Lemma semax_frame_PQR':
+  forall Q2 R2 Espec {cs: compspecs} Delta R1 P Q S c,
+     closed_wrt_modvars c (LOCALx Q2 (SEPx R2)) ->
+     @semax cs Espec Delta (PROPx P (LOCALx Q (SEPx R1))) c
+                     (normal_ret_assert S) ->
+     @semax cs Espec Delta (PROPx P (LOCALx (Q++Q2) (SEPx (R1++R2)))) c
+                     (normal_ret_assert (sepcon S (PROPx nil (LOCALx Q2 (SEPx R2))))).
+Proof.
+intros.
+replace (PROPx P (LOCALx (Q++Q2) (SEPx (R1 ++ R2))))
+   with (PROPx P (LOCALx Q (SEPx (R1))) * (LOCALx Q2 (SEPx R2))).
+eapply semax_pre_post; try (apply semax_frame; try eassumption).
+apply andp_left2; auto.
+apply andp_left2. intro rho; simpl; normalize.
+ unfold PROPx, SEPx, LOCALx, local, lift1.
+normalize.
+simpl; normalize.
+simpl; normalize.
+simpl; normalize.
+clear.
+extensionality rho.
+simpl.
+unfold PROPx, LOCALx, local, lift1, SEPx.
+rewrite fold_right_sepcon_app.
+simpl. normalize.
+f_equal.
+rewrite map_app. rewrite fold_right_and_app.
+apply pred_ext; normalize.
+Qed.
+
+Lemma semax_frame_PQR'':
+  forall Q1 Q2 R1 R2 S1 Espec {cs: compspecs} Delta P Q R S c,
+     closed_wrt_modvars c (LOCALx Q2 (SEPx R2)) ->
+     PROPx P (LOCALx Q (SEPx R)) |-- PROPx P (LOCALx (Q1++Q2) (SEPx (R1++R2))) ->
+     S1 * (PROPx nil (LOCALx Q2 (SEPx R2))) |-- S ->
+     @semax cs Espec Delta (PROPx P (LOCALx Q1 (SEPx R1))) c
+                     (normal_ret_assert S1) ->
+     @semax cs Espec Delta (PROPx P (LOCALx Q (SEPx R))) c
+                     (normal_ret_assert S).
+Proof.
+intros.
+eapply semax_pre_post'; [ | | apply semax_frame_PQR' with (P:=P)].
+apply andp_left2; eassumption.
+apply andp_left2; eassumption.
+auto.
+auto.
+Qed.
+
+Definition __ALLOC : ident := ident_of_string "_ALLOC".
+Definition __LIMIT : ident := ident_of_string "_LIMIT".
+Definition __FRAME : ident := ident_of_string "_FRAME".
+Definition _tinfo : ident := ident_of_string "tinfo".
+Definition _alloc : ident := ident_of_string "alloc".
+Definition _limit : ident := ident_of_string "limit".
+Definition _next : ident := ident_of_string "next".
+Definition _nalloc : ident := ident_of_string "nalloc".
+Definition _save0 : ident := ident_of_string "save0".
+Definition _save1 : ident := ident_of_string "save1".
+Definition _save2 : ident := ident_of_string "save2".
+Definition _save3 : ident := ident_of_string "save3".
+Definition _fp : ident := ident_of_string "fp".
+Definition _prev : ident := ident_of_string "prev".
+Definition _stack_frame : ident := ident_of_string "stack_frame".
+Definition _thread_info : ident := ident_of_string "thread_info".
+Definition _garbage_collect : ident := ident_of_string "garbage_collect".
+Definition ___FRAME__ : ident := ident_of_string "__FRAME__".
+Definition ___ROOT__ : ident := ident_of_string "__ROOT__".
+Definition ___RTEMP__ : ident := ident_of_string "__RTEMP__".
+Definition ___PREV__ : ident := ident_of_string "__PREV__".
+
+
+Definition GC_SAVE1 n := 
+                (Ssequence
+                  (Ssequence
+                    (Sset __LIMIT
+                      (Efield
+                        (Ederef
+                          (Etempvar _tinfo (tptr (Tstruct _thread_info noattr)))
+                          (Tstruct _thread_info noattr)) _limit
+                        (tptr (talignas 3%N (tptr tvoid)))))
+                    (Sset __ALLOC
+                      (Efield
+                        (Ederef
+                          (Etempvar _tinfo (tptr (Tstruct _thread_info noattr)))
+                          (Tstruct _thread_info noattr)) _alloc
+                        (tptr (talignas 3%N (tptr tvoid))))))
+                  (Sifthenelse (Eunop Onotbool
+                                 (Ebinop Ole (Econst_int (Int.repr n) tint)
+                                   (Ebinop Osub
+                                     (Etempvar __LIMIT (tptr (talignas 3%N (tptr tvoid))))
+                                     (Etempvar __ALLOC (tptr (talignas 3%N (tptr tvoid))))
+                                     tlong) tint) tint)
+                    (Ssequence
+                      (Sassign
+                        (Efield
+                          (Ederef
+                            (Etempvar _tinfo (tptr (Tstruct _thread_info noattr)))
+                            (Tstruct _thread_info noattr)) _nalloc tulong)
+                        (Econst_int (Int.repr n) tint))
+                      (Ssequence
+                        (Ssequence
+                          (Ssequence
+                            (Ssequence
+                              (Ssequence
+                                (Ssequence
+                                  (Ssequence
+                                    (Sassign
+                                      (Efield
+                                        (Ederef
+                                          (Etempvar _tinfo (tptr (Tstruct _thread_info noattr)))
+                                          (Tstruct _thread_info noattr)) _fp
+                                        (tptr (Tstruct _stack_frame noattr)))
+                                      (Eaddrof
+                                        (Evar ___FRAME__ (Tstruct _stack_frame noattr))
+                                        (tptr (Tstruct _stack_frame noattr))))
+                                    (Sassign
+                                      (Efield
+                                        (Evar ___FRAME__ (Tstruct _stack_frame noattr))
+                                        _next
+                                        (tptr (talignas 3%N (tptr tvoid))))
+                                      (Ebinop Oadd
+                                        (Evar ___ROOT__ (tarray (talignas 3%N (tptr tvoid)) 1))
+                                        (Econst_int (Int.repr 1) tint)
+                                        (tptr (talignas 3%N (tptr tvoid))))))
+                                  (Sassign
+                                    (Ederef
+                                      (Ebinop Oadd
+                                        (Evar ___ROOT__ (tarray (talignas 3%N (tptr tvoid)) 1))
+                                        (Econst_int (Int.repr 0) tint)
+                                        (tptr (talignas 3%N (tptr tvoid))))
+                                      (talignas 3%N (tptr tvoid)))
+                                    (Etempvar _save0 (talignas 3%N (tptr tvoid)))))
+                                (Scall None
+                                  (Evar _garbage_collect (Tfunction
+                                                           (Tcons
+                                                             (tptr (Tstruct _thread_info noattr))
+                                                             Tnil) tvoid
+                                                           cc_default))
+                                  ((Etempvar _tinfo (tptr (Tstruct _thread_info noattr))) ::
+                                   nil)))
+                              (Sset ___RTEMP__
+                                (Ecast
+                                  (Ecast (Econst_int (Int.repr 0) tint)
+                                    (tptr tvoid))
+                                  (talignas 3%N (tptr tvoid)))))
+                            (Sset _save0
+                              (Ederef
+                                (Ebinop Oadd
+                                  (Evar ___ROOT__ (tarray (talignas 3%N (tptr tvoid)) 1))
+                                  (Econst_int (Int.repr 0) tint)
+                                  (tptr (talignas 3%N (tptr tvoid))))
+                                (talignas 3%N (tptr tvoid)))))
+                          (Sset ___PREV__
+                            (Efield
+                              (Evar ___FRAME__ (Tstruct _stack_frame noattr))
+                              _prev (tptr (Tstruct _stack_frame noattr)))))
+                        (Sassign
+                          (Efield
+                            (Ederef
+                              (Etempvar _tinfo (tptr (Tstruct _thread_info noattr)))
+                              (Tstruct _thread_info noattr)) _fp
+                            (tptr (Tstruct _stack_frame noattr)))
+                          (Etempvar ___PREV__ (tptr (Tstruct _stack_frame noattr))))))
+                    Sskip)).
+
+
+Ltac get_rep_temps ti Q :=
+ lazymatch Q with
+ | nil => constr:(Q)
+ | temp ti ?v :: ?r => let r' := get_rep_temps ti r in constr:(temp ti v :: r')
+ | temp ?i (rep_type_val ?g ?v) :: ?r => 
+    let r' := get_rep_temps ti r in constr:(temp i (rep_type_val g v) :: r')
+ | temp ?i ?v :: ?r => get_rep_temps ti r
+ | ?t :: ?r => let r' := get_rep_temps ti r in constr:(t::r')
+ end.
+
+Ltac get_nonrep_temps ti Q :=
+ lazymatch Q with
+ | nil => constr:(Q)
+ | temp ti _ :: ?r => get_nonrep_temps ti r 
+ | temp ?i (rep_type_val ?g ?v) :: ?r => get_nonrep_temps ti r
+ | temp ?i ?x :: ?r => let r' := get_nonrep_temps ti r in constr:(temp i x ::r')
+ | _ :: ?r => get_nonrep_temps ti r
+ end.
+
+Ltac get_gc_mpreds R :=
+ lazymatch R with
+ | nil => constr:(R)
+ | ?r1 :: ?r => 
+   lazymatch r1 with
+   | full_gc _ _ _ _ _ _ _  => let r' := get_gc_mpreds r in constr:(r1::r')
+   | frame_rep_ _ _ _ _ _ => let r' := get_gc_mpreds r in constr:(r1::r')
+   | library.mem_mgr _ => let r' := get_gc_mpreds r in constr:(r1::r')
+   | is_in_graph _ _ => let r' := get_gc_mpreds r in constr:(r1::r')
+   | _ => get_gc_mpreds r
+   end
+ end.
+
+Ltac get_nongc_mpreds R :=
+ lazymatch R with
+ | nil => constr:(R)
+ | ?r1 :: ?r => 
+   lazymatch r1 with
+   | full_gc _ _ _ _ _ _ _  => get_nongc_mpreds r
+   | frame_rep_ _ _ _ _ _ => get_nongc_mpreds r
+   | library.mem_mgr _ => get_nongc_mpreds r
+   | is_in_graph _ _ => get_nongc_mpreds r
+   | _ => let r' := get_nongc_mpreds r in constr:(r1::r')
+   end
+ end.
+
+Lemma perhaps_gc_1_live_root_aux:
+ forall P Q R Q2 R2,
+  (EX (g': graph) (v0': rep_type) (roots': roots_t) (t_info': GCGraph.thread_info),
+   PROPx (P g' v0' roots' t_info')
+    (LOCALx (Q g' v0' roots' t_info')
+     (SEPx (R g' v0' roots' t_info')))) * (PROPx nil (LOCALx Q2 (SEPx R2))) |--
+  (EX (g': graph) (v0': rep_type) (roots': roots_t) (t_info': GCGraph.thread_info),
+     PROPx (P g' v0' roots' t_info')
+    (LOCALx (Q g' v0' roots' t_info' ++ Q2)
+     (SEPx (R g' v0' roots' t_info' ++ R2)))).
+Proof.
+intros.
+Intros a b c d; Exists a b c d.
+rewrite PROP_combine.
+rewrite app_nil_r.
+auto.
+Qed.
 
 
