examples/bytestring/prims_verif.v
@@ -5,6 +5,12 @@ Require Import CertiGraph.CertiGC.spatial_gcgraph.
 
 Require Import VeriFFI.examples.bytestring.specs.
 
+Lemma representable_string_max_length:
+  forall (s: string) (g: graph) (p: rep_type),
+   is_in_graph g s p ->
+   graph_rep g |-- !! (Z.of_nat (String.length s) < Ptrofs.max_unsigned/4).
+Admitted.
+
 Lemma body_pack:
   semax_body Vprog Gprog f_pack pack_spec.
 Proof.
@@ -20,6 +26,41 @@ Proof.
  forward.
  forward.
  forward.
+ change (temp _temp _) with (temp _temp (rep_type_val g p)).
+ sep_apply (representable_string_max_length x g p); auto.
+ Intros.
+ rewrite Int.signed_repr by rep_lia.
+ sep_apply_compspecs CompSpecs 
+  (frame_rep__fold Tsh v___FRAME__ v___ROOT__ (ti_fp t_info) 1 (Vlong (Int64.repr 0))).
+ sep_apply_compspecs CompSpecs (before_gc_thread_info_rep_fold sh t_info ti).
+ sep_apply (full_gc_fold gv g t_info roots outlier ti sh).
+ forward_loop
+   (EX s:string, EX ps: rep_type,
+     PROP (Z.of_nat (String.length s) <= Z.of_nat (String.length x);
+           is_in_graph g s ps)
+     LOCAL (temp _len (Vlong (Int64.repr 
+               (Z.of_nat (String.length x) - Z.of_nat (String.length s))));
+            temp _temp (rep_type_val g ps);
+            lvar ___FRAME__ (Tstruct _stack_frame noattr) v___FRAME__;
+            lvar ___ROOT__ (tarray int_or_ptr_type 1) v___ROOT__; 
+            gvars gv; temp _tinfo ti; temp _save0 (rep_type_val g p))
+     SEP (full_gc g t_info roots outlier ti sh gv;
+          frame_rep_ Tsh v___FRAME__ v___ROOT__ (ti_fp t_info) 1))
+   break: 
+    (PROP ()
+     LOCAL (temp _len (Vlong (Int64.repr (Z.of_nat (String.length x))));
+            lvar ___FRAME__ (Tstruct _stack_frame noattr) v___FRAME__;
+            lvar ___ROOT__ (tarray int_or_ptr_type 1) v___ROOT__; 
+            gvars gv; temp _tinfo ti; temp _save0 (rep_type_val g p))
+     SEP (full_gc g t_info roots outlier ti sh gv;
+          frame_rep_ Tsh v___FRAME__ v___ROOT__ (ti_fp t_info) 1)).
+ - Exists x p. entailer!!. f_equal. f_equal. lia.
+ - Intros s ps.
+Fail forward_call. (*
+The command has indeed failed with message:
+Tactic failure: Your Gprog contains no funspec with the name
+_get_Coq_Strings_String_string_tag (level 98).
+*)
  Admitted.
 
 (* REMAINDER OF THIS FILE DUPLICATED FROM examples/uint63nat/prims_verif.v *)
