generator/InGraph.v
@@ -299,3 +299,5 @@ Local Obligation Tactic := in_graph_gen_tac.
 (* prove_has_v. *)
 (* prove_monotone. *)
 (* Defined. *)
+
+
